LeanDag.lean
@@ -1,3 +1,4 @@
+import LeanDag.Common.Counting
 import LeanDag.Common.Validators
 import LeanDag.Common.Block
 import LeanDag.Common.Slots
